Have changed the type of WAR variables, changed appropriate updating functions, about to switch from lists to sequences

scrap.v
@@ -258,6 +258,10 @@ checks if a warvar is in the domain, rather than checking a location.
 Inductive array :=
   Array (s: string) (l: nat).
 
+Definition get_length (a: array) :=
+  match a with
+    Array _ length => length end.
+
 Inductive volatility :=
   nonvol
  | vol.
@@ -265,26 +269,54 @@ Inductive volatility :=
 Inductive smallvar :=
   SV (s: string) (q: volatility).
 
-Inductive dangerous_el :=
-  El_d (a: array) (n: value).
+Inductive el_loc :=
+  El (a: array) (i: ('I_(get_length a))).
+
+Definition index_loc (a: array) (i: ('I_(get_length a))) :=
+  El a i.
+
+(*'I_5 the type of all naturals < 5*)
+
+Check (enum _).
+
+Check enum [pred x: 'I_5 | true].
+
+Check enum 'I_5.
+
+
+(*want:
+ do I even have to work with the nats?*)
+
+Compute enum [pred x : 'I_5 | true].
+
+Check [pred x: 'I_5 | x < 3 ].
+
+Check simpl_pred.
+
+Check 'I_4.
+
+Definition test (n: nat) :=
+  'I_n.
+
+
 
 (*used subtypes to enforce the fact that only some expressions are
- memory locations*)
+ memory locations
 Definition elpred  := (fun x=> match x with
-                                        El_d (Array _ length) (Nat i) => (i <? length)
+                                        El (Array _ length) (Nat i) => (i <? length)
                             | _ => false                                            
                             end).
 (*elpred checks if index is a natural in bounds*)
 
-Notation el := {x: dangerous_el | elpred x}.
+Notation el_old := {x: el_loc | elpred x}.
 
-Check SubType el.
+Check SubType el.*)
 
 Inductive exp :=
   Var (x: smallvar) 
 | Val (v: value)
 | Bop (bop: boptype) (e1: exp) (e2: exp) 
-| El_loc (e: el)
+| El_loc (e: el_loc)
 | Element (a: array) (e: exp). (*good that you let in out of bounds arrays here because it means that
                            war bugs of that kind can still get in at the type level,
                            need the CP system*)
@@ -293,9 +325,12 @@ Coercion Var : smallvar >-> exp.
 Notation "a '[[' e ']]'" := (Element (a) (e))
                               (at level 100, right associativity).
 
+Coercion El_loc : el_loc >-> exp.
 
-Definition loc := smallvar + el. (*memory location type*)
+Definition loc := smallvar + el_loc. (*memory location type*)
 
+Definition generate_locs (a: array): list (el_loc) :=
+  map (index_loc a) (enum ('I_(get_length a))).
 Notation warvars := (list loc).
 (*Coercion (inl smallvar el): smallvar >-> loc.*)
 (*Coercion inl: smallvar >-> loc.*)
@@ -342,18 +377,42 @@ Canonical array_eqtype := Eval hnf in EqType array array_eqMixin.
 
 (*equality type for elements*)
 
-Definition eqb_el_d (x y:dangerous_el) :=
+
+Check cast_ord.
+
+
+
+Definition eqb_el_d (x y:el_loc) :=
   match x, y with
-    El_d ax ix, El_d ay iy => (ax==ay) && (ix == iy) end.
+    El ax ix, El ay iy => (ax==ay) && ((nat_of_ord ix) == (nat_of_ord iy)) end.
 
 
-Lemma eqb_eld_iff : forall x y : dangerous_el,
+
+Lemma annoying: forall(a1 a2: array),
+    a1 == a2 -> 'I_(get_length a1) = 'I_(get_length a2).
+by move => a1 a2 / eqP ->. Qed.
+
+
+Set Printing All.
+(*tidy this up*)
+Lemma eqb_eld_iff : forall x y : el_loc,
     is_true(eqb_el_d x y) <-> x = y.
 Proof.
-  case => [ax ix] [ay yP]. simpl.
-  split. case / (reflect_conj eqP eqP) => [H1 H2]. by subst.
-  move => [H1 H2]. subst. apply/ (reflect_conj eqP eqP). auto.
+  case => [ax ix] [ay iy]. simpl.
+  split.   case / (reflect_conj eqP eqP) => [H1 H2]. subst.
+  cut (ix = iy).
+  intros. by subst.
+    by apply val_inj.
+ Unset Printing All.
+ move => [H1 H2].
+ apply andb_true_iff. split.
+   by move / eqP : H1.
+  inversion H2. (*why does this inversion cause a loop?*)
+  by apply (introT eqP).
 Qed.
+
+
+
 
 Lemma eq_eld_iff: Equality.axiom eqb_el_d.
 Proof.
@@ -363,26 +422,14 @@ Proof.
   -  constructor. intros contra. apply eqb_eld_iff in contra.
      rewrite contra in beq. discriminate beq.
 Qed.
-Check el.
-Check val.
 Check SubEqMixin.
 Check EqMixin.
 Check Equality.mixin_of.
 Canonical eld_eqMixin := EqMixin eq_eld_iff.
-Canonical eld_eqtype := Eval hnf in EqType dangerous_el eld_eqMixin.
+Canonical eld_eqtype := Eval hnf in EqType el_loc eld_eqMixin.
 (*suggests it wants an equality relation for the big type before it lets
  you have it for the subtype...that's annoying...ask arthur*)
-Check SubEqMixin.
-Check SubType.
 
-Definition testname := Array "a" 10.
-Definition testname1 := El_d testname 0.
-Lemma xworks: is_true (elpred testname1).
-  unfold elpred. unfold testname1. unfold testname. auto. Qed.
-
-Definition Test: el := eqtype.Sub testname1 xworks. (*ask arthur shouldn't coq be able to infer the subtype type*)
-
-Check Test == Test.
 
 (*smallvar functions*)
 Definition isNV_b (x: smallvar) := (*checks if x is stored in nonvolatile memory*)
@@ -457,56 +504,7 @@ Qed.
 Canonical loc_eqMixin := EqMixin eqloc.
 Canonical loc_eqtype := Eval hnf in EqType loc loc_eqMixin.
 
-Definition get_length (a: array) :=
-  match a with
-    Array _ length => length end.
 
-Definition index (a: array) := 'I_(get_length a).
-
-Definition generate_locs' (a: array): list (index a) := enum (index a).
-
-Check generate_locs'.
-
-
-
-Sub (value) (proof)
-
-Check (enum _).
-
-Check enum [pred x: 'I_5 | x < 3 ]. 
-
-Check [pred x: 'I_5 | x < 3 ].
-
-Check simpl_pred.
-
-
-Lemma annoying: forall(a: array) (n: nat),
-    (n < (get_length a)) -> is_true (elpred (El_d a (Nat n))).
-Admitted.
-
-
-
-Fixpoint generate_locs (a: array) (n: nat) (H: (get_length a) < n) :=
-  match n with
-    0 => [Sub (El_d a (Nat 0)) (annoying H)]
-  | S n' => (Sub (El_d a (Nat n)) (annoying H))::
-                                              generate_locs a n'
-                                              (transitivity term)
-El_d a (Nat n)::(generate_locs a n') end.
-
-Definition array_to_el (a: array) :=
-  match a with
-    Array _ length => generate_locs a length end.
-
-Lemma elpredok: forall(a: array) (x: dangerous_el),
-    In x (array_to_el a) -> is_true (elpred x).
-Admitted.
-
-Definition array_to_loc (a: array) :=
-  map (fun x => el_to_loc (elpredok a) x ___)  (*how to communicate to map
-                                                  that the element it's manipulatin
-                                                  is in the argument list
-                                                  ask arthur*)
 
 (*******************************************************************)
 
@@ -783,11 +781,11 @@ Inductive eeval: nvmem -> vmem -> exp -> readobs -> value -> Prop :=
            (index: exp)
            (rindex: readobs)
            (vindex: value)
-           (element: el)
+           (element: el_loc)
            (v: value),
     eeval N V (index) rindex vindex ->
     ((inr element) <-N) = v ->
-    (val element) = (El_d a vindex) -> (*extra premise to check that inr element
+    (val element) = (El a vindex) -> (*extra premise to check that inr element
                                         is actually a[vindex] *)
 (*well-typedness, valuability, inboundedness of vindex are checked in elpred*)
     (isvaluable v) -> (*extra premise to check if v is valuable*)
@@ -863,7 +861,7 @@ CheckPoint: forall(N: nvmem)
                (element: el),
     eeval N V ei ri vi ->
     eeval N V e r v ->
-    (val element) = (El_d a vi) -> (*extra premise to check that inr element
+    (val element) = (El a vi) -> (*extra premise to check that inr element
                                         is actually a[vindex] *)
 (*well-typedness, valuability, inboundedness of vindex are checked in elpred*)
     (isvaluable v) -> (*extra premise to check if v is valuable*)
@@ -952,7 +950,7 @@ Inductive iceval_w: iconf -> obseq -> iconf -> the_write_stuff -> Prop :=
                (element: el),
     eeval N V ei ri vi ->
     eeval N V e r v ->
-    (val element) = (El_d a vi) -> (*extra premise to check that inr element                                        is actually a[vi] *)
+    (val element) = (El a vi) -> (*extra premise to check that inr element                                        is actually a[vi] *)
 (*well-typedness, valuability, inboundedness of vindex are checked in elpred*)
     (isvaluable v) -> (*extra premise to check if v is valuable*)
     iceval_w (k, N, V, Ins (asgn_arr a ei e))
